[ASL] ACL2 stdlib proofs: reduce boilerplate in loop proofs

asllib/acl2/proofs/stdlib/utils.lisp
@@ -46,7 +46,8 @@
 
 
 ;; Induction scheme for while loops
-(define loop-induct ((env env-p) (clk natp) (test expr-p) (body stmt-p) (whilep) (limit acl2::maybe-integerp) orac)
+(define loop-induct ((env env-p) (whilep) (limit acl2::maybe-integerp) (test expr-p) (body stmt-p)
+                     &key ((clk natp) 'clk) (orac 'orac))
   :verify-guards nil
   :non-executable t
   :measure (nfix clk)
@@ -59,11 +60,11 @@
        ((continuing blkev.res))
        ((when (zp clk))
         blkev.res.env))
-    (loop-induct blkev.res.env (1- clk) test body whilep limit orac)))
+    (loop-induct blkev.res.env whilep limit test body :clk (1- clk))))
 (in-theory (enable (:i loop-induct)))
 
 
-(define for-induct ((env env-p) (index_name identifier-p) (start integerp) (dir for_direction-p) (end integerp) (body stmt-p) (clk natp) (limit acl2::maybe-integerp) orac)
+(define for-induct ((env env-p) (index_name identifier-p) (limit acl2::maybe-integerp) (start integerp) (dir for_direction-p) (end integerp) (body stmt-p) &key ((clk natp) 'clk) (orac 'orac))
   :verify-guards nil
   :non-executable t
   :measure (for_loop-measure start end dir)
@@ -73,7 +74,7 @@
        ((mv (ev_normal blkev) orac) (eval_block env body))
        ((continuing blkev.res))
        ((mv step env2) (eval_for_step blkev.res.env index_name start dir)))
-    (for-induct env2 index_name step dir end body clk limit orac)))
+    (for-induct env2 index_name limit step dir end body)))
 (in-theory (enable (:i for-induct)))
 
     
@@ -128,3 +129,322 @@
 
 
 
+
+
+                    
+                       
+(program)
+
+(defun loop-local-var-bindings (local-vars)
+  (if (atom local-vars)
+      nil
+    (let* ((rest (loop-local-var-bindings (cdr local-vars)))
+           (first (car local-vars)))
+      (case-match first
+        (((ctor name) str . &)
+         (if (and (stringp str)
+                  (member ctor '(v_int v_bool v_real v_string v_bitvector v_label v_record v_array))
+                  (symbolp name))
+             (append (acl2::template-subst '((<name>-look (hons-assoc-equal <str> env.local.storage))
+                                             ((<ctor> <name>) (cdr <name>-look)))
+                                           :atom-alist `((<ctor> . ,ctor)
+                                                         (<name> . ,name)
+                                                         (<str> . ,str))
+                                           :str-alist `(("<NAME>" . ,(symbol-name name)))
+                                           :pkg-sym 'asl-pkg)
+                     rest)
+           (er hard? 'loop-local-var-bindings "Bad local-vars entry: ~x0" first)))
+        (& (er hard? 'loop-local-var-bindings "Bad local-vars entry: ~x0" first))))))
+
+;; (loop-local-var-bindings '(((v_bitvector x) "__stdlib_local_x") ((v_int n) "__stdlib_local_N")))
+
+(defun loop-local-var-hyps (local-vars)
+  (if (atom local-vars)
+      nil
+    (let* ((rest (loop-local-var-hyps (cdr local-vars)))
+           (first (car local-vars)))
+      (case-match first
+        (((ctor name) & . &)
+         (append (acl2::template-subst '(<name>-look
+                                         (val-case <name> <kind>))
+                                       :atom-alist `((<kind> . ,(intern-in-package-of-symbol
+                                                                 (symbol-name ctor) :keyword-pkg))
+                                                     (<name> . ,name))
+                                       :str-alist `(("<NAME>" . ,(symbol-name name)))
+                                       :pkg-sym 'asl-pkg)
+                 rest))
+        (& rest)))))
+
+(defun loop-local-vars-final-env (local-vars)
+  (if (atom local-vars)
+      'env.local.storage
+    (let* ((rest (loop-local-vars-final-env (cdr local-vars)))
+           (first (car local-vars)))
+      (case-match first
+        ((& str final-val)
+         `(put-assoc-equal ,str ,final-val ,rest))
+        (& rest)))))
+
+;; (loop-local-var-hyps '(((v_bitvector x) "__stdlib_local_x") ((v_int n) "__stdlib_local_N")))
+
+
+
+(defconst *defloop-template*
+  '(defsection <name>
+     (defconst *<name>*
+       (find-nth-form <nth> <looptype>
+                      (hons-assoc-equal <fn>
+                                        (static_env_global->subprograms <static-env>))))
+
+     (:@ (not :s_for)
+      (defconst *<name>-test*
+        (<looptype>->test *<name>*)))
+
+     (defconst *<name>-body*
+       (<looptype>->body *<name>*))
+
+     <prepwork>
+     
+     (local (in-theory (acl2::e/d* (<defloop-enables>
+                                    <user-enables>)
+                                   (<defloop-disables>
+                                    <user-disables>))))
+     (defthm <name>-correct
+       (b* (((env env))
+            ((local-env env.local))
+            <local-var-bindings>
+            <user-bindings>)
+         (implies (and <local-var-hyps>
+                       ;; <measure-hyps>
+                       <invariants>
+                       (no-duplicatesp-equal (acl2::alist-keys env.local.storage)))
+                  (b* (((mv (ev_normal res) &) <loop-form>))
+                    <concl>)))
+       :hints (;; copied from just-induct-and-expand
+               (if (equal (car id) '(0))
+                   (let* ((expand-hints (acl2::just-expand-cp-parse-hints
+                                         '(<loop-form-expand>) (w state)))
+                          (cproc `(acl2::mark-expands-cp clause '(nil t ,expand-hints))))
+                     `(:computed-hint-replacement
+                       ((and (equal (car id) '(0)) '(:clause-processor acl2::clause-to-term))
+                        (and (equal (car id) '(0)) '(:induct <induction>)))
+                       :clause-processor ,cproc))
+                 (and (equal (car id) '(0 1))
+                      (acl2::expand-marked :last-only t)))
+               <user-hints>))))
+
+
+
+
+
+(define defloop-fn (name args state)
+  (b* (((std::extract-keyword-args
+         :other-args bad-args
+         ;; :kwd-alist kwd-alist
+         function
+         (looptype :while)
+         (nth 0)
+
+         ;; format: ((val_type acl2-varname) "asl-varname" [ final value ] )* --
+         ;; e.g. (((v_bitvector x) "__stdlib_local_x" x-final-value) ((v_int n) "__stdlib_local_N"))
+         ;; For loop index is separately listed as index-var
+         local-vars
+         index-var
+         (start-var 'start)
+         (end-var 'end)
+
+         ;; For now we just support loops that execute normally (no
+         ;; throw/error) -- eventually add conditions for throwing/erroring.
+
+         ;; When loop finishes (continuing), then the local-vars above give the
+         ;; final values stored in the updated environment. If it returns
+         ;; early, we need to know the return condition and return values.
+         (return-cond 'nil)
+         return-values
+         
+         enable
+         disable
+         hints
+         prepwork
+         
+         (invariants 't)
+         bindings
+         (static-env '(stdlib-static-env)))
+        args)
+       ((when bad-args)
+        (er soft 'defloop "Bad arguments: ~x0" bad-args))
+       ((unless (stringp function))
+        (er soft 'defloop "Function should be a string: ~x0" function))
+       (orig-looptype looptype)
+       (looptype (case orig-looptype
+                   ((:while :s_while) :s_while)
+                   ((:for :s_for) :s_for)
+                   ((:repeat :s_repeat) :s_repeat)
+                   (t nil)))
+       ((unless looptype)
+        (er soft 'defloop "Bad looptype: ~x0" orig-looptype))
+       ((unless (natp nth))
+        (er soft 'defloop "Bad nth: ~x0" nth))
+       ((acl2::er (cons & static-env-val))
+        (acl2::simple-translate-and-eval static-env nil nil
+                                         (msg "static env ~x0" static-env)
+                                         'defloop (w state) state t))
+       ((unless (static_env_global-p static-env-val))
+        (er soft 'defloop "Bad static env (evaluation of ~x0): doesn't satisfy static_env_global-p" static-env))
+       (fn-struct (hons-assoc-equal function
+                                    (static_env_global->subprograms static-env-val)))
+       ((unless fn-struct)
+        (er soft 'defloop "Bad function ~x0: not found in static env" function))
+       ;; if found, then it's the right type
+       (form (find-nth-form nth looptype fn-struct))
+       ((unless form)
+        (er soft 'defloop "Loop not found: function ~x0 looptype ~x1 nth ~x2" function looptype nth))
+
+       ((when (and (eq looptype :s_for)
+                   (not index-var)))
+        (er soft 'defloop "Index var must be specified for for loops"))
+       ((when (and index-var (not (eq looptype :s_for))))
+        (er soft 'defloop "Index var specified for non-for loop"))
+       
+       (local-vars (if (eq looptype :s_for)
+                       (cons `((v_int ,index-var)
+                               ,(s_for->index_name form)
+                               (v_int
+                                ,(if (eq (s_for->dir form) :up)
+                                     `(+ 1 ,end-var)
+                                   `(+ -1 ,end-var))))
+                             local-vars)
+                     local-vars))
+                               
+       (local-var-bindings (loop-local-var-bindings local-vars))
+       (local-var-hyps (loop-local-var-hyps local-vars))
+       (local-var-hyps (if (eq looptype :s_for)
+                           (append local-var-hyps
+                                   `((equal (v_int->val ,index-var) ,start-var)
+                                     (integerp ,end-var)
+                                     ,(if (eq (s_for->dir form) :up)
+                                          `(<= ,start-var (+ 1 ,end-var))
+                                        `(<= (+ -1 ,end-var) ,start-var))))
+                         local-var-hyps))
+        
+       (local-var-final-env (loop-local-vars-final-env local-vars))
+
+       (continuing-concl
+        `(and (equal (control_flow_state-kind res.res) :continuing)
+              (b* (((continuing res.res)))
+                (equal res.res.env
+                       (change-env env
+                                   :local
+                                   (change-local-env
+                                    env.local
+                                    :storage ,local-var-final-env))))))
+       (returning-concl
+        `(and (equal (control_flow_state-kind res.res) :returning)
+              (b* (((returning res.res)))
+                (and (equal res.res.vals ,return-values)
+                     (equal res.res.env env.global)))))
+
+       (normal-concl
+        `(and (equal (eval_result-kind res) :ev_normal)
+              ,@(and (not (eq return-cond t))
+                     `(,(if (eq return-cond nil)
+                            continuing-concl
+                          `(implies (not ,return-cond)
+                                    ,continuing-concl))))
+              ,@(and (not (eq return-cond nil))
+                     `(,(if (eq return-cond t)
+                            returning-concl
+                          `(implies ,return-cond
+                                    ,returning-concl))))))
+                       
+              
+       ((acl2::tmplsubst template)
+        (acl2::make-tmplsubst
+         :atoms `((<name> . ,name)
+                  (<nth> . ,nth)
+                  (<looptype> . ,looptype)
+                  (<fn> . ,function)
+                  (<static-env> . ,static-env)
+                  (<invariants> . ,invariants)
+                  (<concl> . ,normal-concl))
+         :splices `((<defloop-enables> . (defloop-enables))
+                    (<defloop-disables> . (defloop-disables))
+                    (<user-enables> . ,enable)
+                    (<user-disables> . ,disable)
+                    (<local-var-bindings> . ,local-var-bindings)
+                    (<local-var-hyps> . ,local-var-hyps)
+                    (<user-hints> . ,hints)
+                    (<user-bindings> . ,bindings)
+                    (<prepwork> . ,prepwork))
+         :strs `(("<NAME>" . ,(symbol-name name))
+                 ("<LOOPTYPE>" . ,(symbol-name looptype)))
+         :features (list looptype)
+         :pkg-sym 'asl-pkg))
+
+       (body-const (acl2::template-subst-top '*<name>-body* template))
+       (test-const (acl2::template-subst-top '*<name>-test* template))
+       
+       ((mv loop-form expand induction)
+        (case looptype
+          (:s_for
+           (let ((args `(env ,(s_for->index_name form)
+                             ,(and (s_for->limit form) 'limit)
+                             ,start-var ,(s_for->dir form) ,end-var
+                             ,body-const)))
+             (mv `(eval_for  . ,args)
+                 `(:free (limit ,start-var ,end-var)
+                   (eval_for . ,args))
+                 `(for-induct . ,args))))
+          (t
+           (let ((args `(env ,(eq looptype :s_while)
+                             ,(and (if (eq looptype :s_while)
+                                       (s_while->limit form)
+                                     (s_repeat->limit form))
+                                   'limit)
+                             ,test-const ,body-const)))
+             (mv `(eval_loop . ,args)
+                 `(:free (limit) (eval_loop . ,args))
+                 `(loop-induct . ,args))))))
+
+       (template (acl2::change-tmplsubst
+                  template :atoms `((<loop-form> . ,loop-form)
+                                    (<induction> . ,induction)
+                                    (<loop-form-expand> . ,expand)
+                                    . ,template.atoms)))
+                      
+                      
+       (event
+        (acl2::template-subst-top *defloop-template* template)))
+    (value event)))
+
+(defmacro defloop (name &rest args)
+  `(make-event (defloop-fn ',name ',args state)))
+
+
+
+
+(acl2::def-ruleset! defloop-enables '(check_recurse_limit
+                                      declare_local_identifiers
+                                      declare_local_identifier
+                                      env-find
+                                      env-assign
+                                      env-assign-local
+                                      env-assign-global
+                                      env-push-stack
+                                      env-pop-stack
+                                      pop_scope
+                                      tick_loop_limit
+                                      v_to_bool
+                                      eval_for_step
+                                      for_loop-step
+                                      for_loop-test
+                                      check-bad-slices
+                                      slices_sub
+                                      check_non_overlapping_slices
+                                      check_non_overlapping_slices-1
+                                      slices-width
+                                      write_to_bitvector
+                                      write_to_bitvector-aux
+                                      vbv-to-int))
+
+(acl2::def-ruleset defloop-disables nil)
