asllib/acl2/proofs/stdlib/log2.lisp
@@ -34,470 +34,125 @@
                            put-assoc-equal
                            hons-assoc-equal)))
 
-(defsection log2-loop
 
-  (defconst *log2-loop*
-    (find-nth-form 0 :s_while (assoc-equal "Log2" (static_env_global->subprograms
-                                                    (stdlib-static-env)))))
-
-  (defconst *log2-loop-test*
-    (s_while->test *log2-loop*))
-
-  (defconst *log2-loop-body*
-    (s_while->body *log2-loop*))
-
-  ;; (local (defthm ratonal-exponent-of-equal-to-expt-2
-  ;;          (implies (equal x (expt 2 n))
-  ;;                   (equal (acl2::rational-exponent x)
-  ;;                          (ifix n)))))
-
-
-  (local (Defthmd rational-exponent-unique-of-nonneg
-           (implies (and (<= (expt 2 r) a)
-                         (< a (* 2 (expt 2 r)))
-                         (integerp a)
-                         (integerp r))
-                    (equal (acl2::rational-exponent a) r))
-           :hints (("goal" :use ((:instance acl2::rational-sign-significand-exponent-unique
-                                  (sign 1) (significand (/ a (expt 2 r))) (exponent r)))))))
-  
-  (local (defthm rational-exponent-hack
-           (implies (and (<= a (expt 2 r))
-                         (< (expt 2 r) (* 2 a))
-                         (integerp a)
-                         (integerp r))
-                    (equal r (if (equal a (expt 2 r))
-                                 (acl2::rational-exponent a)
-                               (+ 1 (acl2::rational-exponent a)))))
-           :hints (("goal" :do-not-induct t
-                    :expand ((:free (x) (hide x))))
-                   (and stable-under-simplificationp
-                        '(:use ((:instance rational-exponent-unique-of-nonneg
-                                 (r (+ -1 r))))
-                          :expand ((expt 2 r)))))
-           :otf-flg t
-           :rule-classes nil))
-                         
-
-  (local (defthm put-assoc-equal-identity-free
-           (implies (and (equal v (cdr (hons-assoc-equal k x)))
-                         (hons-assoc-equal k x)
-                         (alistp x))
-                    (equal (put-assoc-equal k v x) x))))
-
-  ;; (local (defthmd equal-of-v_int->val
-  ;;          (implies (val-case x :v_int)
-  ;;                   (equal (equal (v_int->val x) y)
-  ;;                          (and (integerp y)
-  ;;                               (equal (val-fix x) (v_int y)))))))
-
-                         
-  
-  (local (defthmd equal-when-v_int
-           (implies (and (val-case x :v_int)
-                         (val-case y :v_int)
-                         (val-p x) (val-p y))
-                    (equal (equal x y)
-                           (equal (v_int->val x)
-                                  (v_int->val y))))
-           :hints (("goal" :use ((:instance val-fix-when-v_int (x x))
-                                 (:instance val-fix-when-v_int (x y)))
-                    :in-theory (disable v_int-of-fields
-                                        equal-of-v_int)))))
-
-
-
-
-  (local (defthmd powers-of-2-not-between-lemma1
-           (implies (and (< (ifix ye) (ifix xe))
-                         (<= (ifix ye) 0))
-                    (<= (* 2 (expt 2 ye)) (expt 2 xe)))
-           :hints (("goal" :induct (expt 2 ye)))
-           :otf-flg t))
-  (local (defthmd powers-of-2-not-between-lemma
-           (implies (< (ifix ye) (ifix xe))
-                    (<= (* 2 (expt 2 ye)) (expt 2 xe)))
-           :hints (("goal" :cases ((<= 0 (ifix ye)))
-                    :in-theory (enable powers-of-2-not-between-lemma1)))
-           :otf-flg t))  
-
-  (local (defthm powers-of-2-not-between
-           (implies (< (expt 2 xe) (* 2 (expt 2 ye)))
-                    (<= (expt 2 xe) (expt 2 ye)))
-           :hints (("goal" :use ((:instance acl2::expt-is-increasing-for-base>1
-                                  (r 2) (i (ifix xe)) (j (ifix ye)))
-                                 (:instance acl2::expt-is-increasing-for-base>1
-                                  (r 2) (i (ifix ye)) (j (ifix xe)))
-                                 powers-of-2-not-between-lemma)
-                    :in-theory (acl2::e/d* (acl2::arith-equiv-forwarding)
-                                           (acl2::expt-is-increasing-for-base>1))))
-           :rule-classes nil))
-  
-  ;; (local (defthmd equal-when-powers-of-2
-  ;;          (implies (and (equal x (expt 2 xe))
-  ;;                        (equal y (expt 2 ye))
-  ;;                        (< x (* 2 y)))
-  ;;                   (equal (< x y)
-  ;;                          (not (equal x y))))
-  ;;          :hints (("goal" :do-not-induct t
-  ;;                   :use ((:instance ACL2::EXPT-IS-INCREASING-FOR-BASE>1
-  ;;                          (r 2) (i (ifix ye)) (j (ifix xe)))
-  ;;                         (:instance ACL2::EXPT-IS-INCREASING-FOR-BASE>1
-  ;;                          (r 2) (i (ifix xe)) (j (ifix ye))))
-  ;;                   :in-theory (acl2::e/d* (acl2::arith-equiv-forwarding)
-  ;;                                          (acl2::expt-is-increasing-for-base>1))))
-  ;;          :otf-flg t))
-
-  (local (defthm v_int->val-rewrite-to-exponent
-           (implies (equal (v_int->val x) (expt 2 y))
-                    (equal (v_int->val x) (expt 2 y)))))
-  
-  (defthm log2-loop-correct
-    (b* ((storage (local-env->storage
-                   (env->local env)))
-         (a-look (assoc-equal "__stdlib_local_a" storage))
-         (a (cdr a-look))
-         ((v_int a))
-         (current-look (assoc-equal "__stdlib_local_current" storage))
-         (current (cdr current-look))
-         ((v_int current))
-         (result-look (assoc-equal "__stdlib_local_result" storage))
-         (result (cdr result-look))
-         ((v_int result)))
-      (implies (and a-look
-                    (val-case a :v_int)
-                    current-look
-                    (val-case current :v_int)
-                    result-look
-                    (val-case result :v_int)
-                    (<= 0 result.val)
-                    (equal current.val (expt 2 result.val))
-                    (< current.val (* 2 a.val))
-                    (natp clk)
-                    (< (- (+ 1 (acl2::rational-exponent a.val)) result.val) clk)
-                    (integerp limit)
-                    (< (- (+ 1 (acl2::rational-exponent a.val)) result.val) limit)
-                    (no-duplicatesp-equal (acl2::alist-keys storage)))
-               (b* (((mv (ev_normal res) &) (eval_loop env t limit *log2-loop-test* *log2-loop-body*))
-                    ((continuing res.res))
-                    (result-spec (let ((exp (acl2::rational-exponent a.val)))
-                                   (if (equal a.val (expt 2 exp))
-                                       exp
-                                     (+ 1 exp))))
-                    (current-spec (expt 2 result-spec))
-                    ((env env))
-                    ((local-env env.local)))
-                 (and (equal (eval_result-kind res) :ev_normal)
-                      (equal (control_flow_state-kind res.res) :continuing)
-                      (equal res.res.env
-                             (change-env env
-                                         :local (change-local-env
-                                                 env.local
-                                                 :storage (put-assoc-equal "__stdlib_local_current"
-                                                                           (v_int current-spec)
-                                                                           (put-assoc-equal "__stdlib_local_result"
-                                                                                            (v_int result-spec)
-                                                                                            env.local.storage)))))))))
-    :hints (("goal" :induct (loop-induct env clk *log2-loop-test* *log2-loop-body* t limit orac)
-             :in-theory (enable check_recurse_limit
-                                declare_local_identifiers
-                                declare_local_identifier
-                                env-find
-                                env-assign
-                                env-assign-local
-                                env-assign-global
-                                env-push-stack
-                                env-pop-stack
-                                pop_scope
-                                tick_loop_limit
-                                v_to_bool)
-             :do-not-induct t)
-            (and stable-under-simplificationp
-                 '(:expand ((eval_loop env t limit *log2-loop-test* *log2-loop-body*))))
-            (and stable-under-simplificationp
-                 '(:use ((:instance rational-exponent-hack
-                          (a (V_INT->VAL
-                              (CDR (HONS-ASSOC-EQUAL "__stdlib_local_a"
-                                                     (LOCAL-ENV->STORAGE (ENV->LOCAL ENV))))))
-                          (r (V_INT->VAL
-                              (CDR (HONS-ASSOC-EQUAL "__stdlib_local_result"
-                                                     (LOCAL-ENV->STORAGE (ENV->LOCAL ENV)))))))
-                         (:instance powers-of-2-not-between
-                          (xe (V_INT->VAL
-                               (CDR (HONS-ASSOC-EQUAL "__stdlib_local_result"
-                                                      (LOCAL-ENV->STORAGE (ENV->LOCAL ENV))))))
-                          (ye (acl2::rational-exponent
-                               (V_INT->VAL
-                                (CDR (HONS-ASSOC-EQUAL "__stdlib_local_a"
-                                                       (LOCAL-ENV->STORAGE (ENV->LOCAL ENV))))))))
-                         (:instance rational-exponent-when-expt-less
-                          (i (V_INT->VAL
-                               (CDR (HONS-ASSOC-EQUAL "__stdlib_local_result"
-                                                      (LOCAL-ENV->STORAGE (ENV->LOCAL ENV))))))
-                          (x (V_INT->VAL
+(defloop log2-loop
+  :function "Log2"
+  :looptype :s_while
+  :local-vars (((v_int a)       "__stdlib_local_a")
+               ((v_int current) "__stdlib_local_current" (v_int current-spec))
+               ((v_int result)  "__stdlib_local_result"  (v_int result-spec)))
+  :bindings ((result-spec (let ((exp (acl2::rational-exponent a.val)))
+                            (if (equal a.val (expt 2 exp))
+                                exp
+                              (+ 1 exp))))
+             (current-spec (expt 2 result-spec)))
+  :invariants (and (<= 0 result.val)
+                   (equal current.val (expt 2 result.val))
+                   (< current.val (* 2 a.val))
+                   (< (- (+ 1 (acl2::rational-exponent a.val)) result.val) (ifix clk))
+                   (integerp limit)
+                   (< (- (+ 1 (acl2::rational-exponent a.val)) result.val) limit))
+  :hints ((and stable-under-simplificationp
+               '(:use ((:instance rational-exponent-hack
+                        (a (V_INT->VAL
+                            (CDR (HONS-ASSOC-EQUAL "__stdlib_local_a"
+                                                   (LOCAL-ENV->STORAGE (ENV->LOCAL ENV))))))
+                        (r (V_INT->VAL
+                            (CDR (HONS-ASSOC-EQUAL "__stdlib_local_result"
+                                                   (LOCAL-ENV->STORAGE (ENV->LOCAL ENV)))))))
+                       (:instance powers-of-2-not-between
+                        (xe (V_INT->VAL
+                             (CDR (HONS-ASSOC-EQUAL "__stdlib_local_result"
+                                                    (LOCAL-ENV->STORAGE (ENV->LOCAL ENV))))))
+                        (ye (acl2::rational-exponent
+                             (V_INT->VAL
                               (CDR (HONS-ASSOC-EQUAL "__stdlib_local_a"
                                                      (LOCAL-ENV->STORAGE (ENV->LOCAL ENV))))))))
-                   :in-theory (e/d (equal-when-v_int)
-                                   (rational-exponent-when-expt-less))))
-            ;; (and stable-under-simplificationp
-            ;;      '(:in-theory (e/d (equal-when-v_int)
-            ;;                        (rational-exponent-hack))))
-            ;; (and stable-under-simplificationp
-            ;;      '(:in-theory (e/d (equal-of-v_int->val)
-            ;;                        (equal-of-v_int))))
-            )))
-
-
-
-(defsection log2-loop
-
-  (defconst *log2-loop*
-    (find-nth-form 0 :s_while (assoc-equal "Log2" (static_env_global->subprograms
-                                                    (stdlib-static-env)))))
-
-  (defconst *log2-loop-test*
-    (s_while->test *log2-loop*))
-
-  (defconst *log2-loop-body*
-    (s_while->body *log2-loop*))
-
-  ;; (local (defthm ratonal-exponent-of-equal-to-expt-2
-  ;;          (implies (equal x (expt 2 n))
-  ;;                   (equal (acl2::rational-exponent x)
-  ;;                          (ifix n)))))
-
-
-  (local (Defthmd rational-exponent-unique-of-nonneg
-           (implies (and (<= (expt 2 r) a)
-                         (< a (* 2 (expt 2 r)))
-                         (integerp a)
-                         (integerp r))
-                    (equal (acl2::rational-exponent a) r))
-           :hints (("goal" :use ((:instance acl2::rational-sign-significand-exponent-unique
-                                  (sign 1) (significand (/ a (expt 2 r))) (exponent r)))))))
+                       (:instance rational-exponent-when-expt-less
+                        (i (V_INT->VAL
+                            (CDR (HONS-ASSOC-EQUAL "__stdlib_local_result"
+                                                   (LOCAL-ENV->STORAGE (ENV->LOCAL ENV))))))
+                        (x (V_INT->VAL
+                            (CDR (HONS-ASSOC-EQUAL "__stdlib_local_a"
+                                                   (LOCAL-ENV->STORAGE (ENV->LOCAL ENV))))))))
+                 :in-theory (e/d (equal-when-v_int)
+                                 (rational-exponent-when-expt-less)))))
+  :prepwork
+  ((local (Defthmd rational-exponent-unique-of-nonneg
+            (implies (and (<= (expt 2 r) a)
+                          (< a (* 2 (expt 2 r)))
+                          (integerp a)
+                          (integerp r))
+                     (equal (acl2::rational-exponent a) r))
+            :hints (("goal" :use ((:instance acl2::rational-sign-significand-exponent-unique
+                                   (sign 1) (significand (/ a (expt 2 r))) (exponent r)))))))
   
-  (local (defthm rational-exponent-hack
-           (implies (and (<= a (expt 2 r))
-                         (< (expt 2 r) (* 2 a))
-                         (integerp a)
-                         (integerp r))
-                    (equal r (if (equal a (expt 2 r))
-                                 (acl2::rational-exponent a)
-                               (+ 1 (acl2::rational-exponent a)))))
-           :hints (("goal" :do-not-induct t
-                    :expand ((:free (x) (hide x))))
-                   (and stable-under-simplificationp
-                        '(:use ((:instance rational-exponent-unique-of-nonneg
-                                 (r (+ -1 r))))
-                          :expand ((expt 2 r)))))
-           :otf-flg t
-           :rule-classes nil))
+   (local (defthm rational-exponent-hack
+            (implies (and (<= a (expt 2 r))
+                          (< (expt 2 r) (* 2 a))
+                          (integerp a)
+                          (integerp r))
+                     (equal r (if (equal a (expt 2 r))
+                                  (acl2::rational-exponent a)
+                                (+ 1 (acl2::rational-exponent a)))))
+            :hints (("goal" :do-not-induct t
+                     :expand ((:free (x) (hide x))))
+                    (and stable-under-simplificationp
+                         '(:use ((:instance rational-exponent-unique-of-nonneg
+                                  (r (+ -1 r))))
+                           :expand ((expt 2 r)))))
+            :otf-flg t
+            :rule-classes nil))
                          
 
-  (local (defthm put-assoc-equal-identity-free
-           (implies (and (equal v (cdr (hons-assoc-equal k x)))
-                         (hons-assoc-equal k x)
-                         (alistp x))
-                    (equal (put-assoc-equal k v x) x))))
-  (local (in-theory (disable acl2::put-assoc-equal-identity)))
+   (local (defthm put-assoc-equal-identity-free
+            (implies (and (equal v (cdr (hons-assoc-equal k x)))
+                          (hons-assoc-equal k x)
+                          (alistp x))
+                     (equal (put-assoc-equal k v x) x))))
 
-  ;; (local (defthmd equal-of-v_int->val
-  ;;          (implies (val-case x :v_int)
-  ;;                   (equal (equal (v_int->val x) y)
-  ;;                          (and (integerp y)
-  ;;                               (equal (val-fix x) (v_int y)))))))
+   (local (defthmd powers-of-2-not-between-lemma1
+            (implies (and (< (ifix ye) (ifix xe))
+                          (<= (ifix ye) 0))
+                     (<= (* 2 (expt 2 ye)) (expt 2 xe)))
+            :hints (("goal" :induct (expt 2 ye)))
+            :otf-flg t))
+   (local (defthmd powers-of-2-not-between-lemma
+            (implies (< (ifix ye) (ifix xe))
+                     (<= (* 2 (expt 2 ye)) (expt 2 xe)))
+            :hints (("goal" :cases ((<= 0 (ifix ye)))
+                     :in-theory (enable powers-of-2-not-between-lemma1)))
+            :otf-flg t))  
 
-                         
-  
-  (local (defthmd equal-when-v_int
-           (implies (and (syntaxp (and (not (case-match x (('val-kind$inline . &) t)))
-                                       (not (case-match y (('val-kind$inline . &) t)))))
-                         (val-case x :v_int)
-                         (val-case y :v_int)
-                         (val-p x) (val-p y))
-                    (equal (equal x y)
-                           (equal (v_int->val x)
-                                  (v_int->val y))))
-           :hints (("goal" :use ((:instance val-fix-when-v_int (x x))
-                                 (:instance val-fix-when-v_int (x y)))
-                    :in-theory (disable v_int-of-fields
-                                        equal-of-v_int)))))
-
-  (local (in-theory (disable equal-of-v_int)))
+   (local (defthm powers-of-2-not-between
+            (implies (< (expt 2 xe) (* 2 (expt 2 ye)))
+                     (<= (expt 2 xe) (expt 2 ye)))
+            :hints (("goal" :use ((:instance acl2::expt-is-increasing-for-base>1
+                                   (r 2) (i (ifix xe)) (j (ifix ye)))
+                                  (:instance acl2::expt-is-increasing-for-base>1
+                                   (r 2) (i (ifix ye)) (j (ifix xe)))
+                                  powers-of-2-not-between-lemma)
+                     :in-theory (acl2::e/d* (acl2::arith-equiv-forwarding)
+                                            (acl2::expt-is-increasing-for-base>1))))
+            :rule-classes nil))
 
 
-  (local (defthmd powers-of-2-not-between-lemma1
-           (implies (and (< (ifix ye) (ifix xe))
-                         (<= (ifix ye) 0))
-                    (<= (* 2 (expt 2 ye)) (expt 2 xe)))
-           :hints (("goal" :induct (expt 2 ye)))
-           :otf-flg t))
-  (local (defthmd powers-of-2-not-between-lemma
-           (implies (< (ifix ye) (ifix xe))
-                    (<= (* 2 (expt 2 ye)) (expt 2 xe)))
-           :hints (("goal" :cases ((<= 0 (ifix ye)))
-                    :in-theory (enable powers-of-2-not-between-lemma1)))
-           :otf-flg t))  
+   (local (defthm v_int->val-rewrite-to-exponent
+            (implies (equal (v_int->val x) (expt 2 y))
+                     (equal (v_int->val x) (expt 2 y)))))
 
-  (local (defthm powers-of-2-not-between
-           (implies (< (expt 2 xe) (* 2 (expt 2 ye)))
-                    (<= (expt 2 xe) (expt 2 ye)))
-           :hints (("goal" :use ((:instance acl2::expt-is-increasing-for-base>1
-                                  (r 2) (i (ifix xe)) (j (ifix ye)))
-                                 (:instance acl2::expt-is-increasing-for-base>1
-                                  (r 2) (i (ifix ye)) (j (ifix xe)))
-                                 powers-of-2-not-between-lemma)
-                    :in-theory (acl2::e/d* (acl2::arith-equiv-forwarding)
-                                           (acl2::expt-is-increasing-for-base>1))))
-           :rule-classes nil))
+   (local (defthmd equal-when-v_int
+            (implies (and (val-case x :v_int)
+                          (val-case y :v_int)
+                          (val-p x) (val-p y))
+                     (equal (equal x y)
+                            (equal (v_int->val x)
+                                   (v_int->val y))))
+            :hints (("goal" :use ((:instance val-fix-when-v_int (x x))
+                                  (:instance val-fix-when-v_int (x y)))
+                     :in-theory (disable v_int-of-fields
+                                         equal-of-v_int)))))))
 
-  (local (defthm powers-of-2-not-between-rw
-           (implies (and (equal y (expt 2 ye))
-                         (> (expt 2 xe) (expt 2 ye)))
-                    (>= (expt 2 xe) (* 2 y)))
-           :hints (("goal" :use powers-of-2-not-between
-                    :do-not-induct t))))
-  
-  ;; (local (defthmd equal-when-powers-of-2
-  ;;          (implies (and (equal x (expt 2 xe))
-  ;;                        (equal y (expt 2 ye))
-  ;;                        (< x (* 2 y)))
-  ;;                   (equal (< x y)
-  ;;                          (not (equal x y))))
-  ;;          :hints (("goal" :do-not-induct t
-  ;;                   :use ((:instance ACL2::EXPT-IS-INCREASING-FOR-BASE>1
-  ;;                          (r 2) (i (ifix ye)) (j (ifix xe)))
-  ;;                         (:instance ACL2::EXPT-IS-INCREASING-FOR-BASE>1
-  ;;                          (r 2) (i (ifix xe)) (j (ifix ye))))
-  ;;                   :in-theory (acl2::e/d* (acl2::arith-equiv-forwarding)
-  ;;                                          (acl2::expt-is-increasing-for-base>1))))
-  ;;          :otf-flg t))
-
-  (defund is-same-as (x y)
-    (equal x y))
-  
-  (local (defthm rewrite-equal-of-current->val
-           (b* ((current-look (hons-assoc-equal "__stdlib_local_current" storage))
-                (current (cdr current-look))
-                ((v_int current))
-                (result-look (hons-assoc-equal "__stdlib_local_result" storage))
-                (result (cdr result-look))
-                ((v_int result)))
-             (equal (equal current.val (expt 2 result.val))
-                    (is-same-as current.val (expt 2 result.val))))
-           :hints(("Goal" :in-theory (enable is-same-as)))))
-
-  (local (defthm rewrite-current->val-when-same-as
-           (b* ((current-look (hons-assoc-equal "__stdlib_local_current" storage))
-                (current (cdr current-look))
-                ((v_int current))
-                (result-look (hons-assoc-equal "__stdlib_local_result" storage))
-                (result (cdr result-look))
-                ((v_int result)))
-             (implies (is-same-as current.val (expt 2 result.val))
-                      (equal current.val (expt 2 result.val))))
-           :hints(("Goal" :in-theory (e/d (is-same-as)
-                                          (rewrite-equal-of-current->val))))))
-
-  (local (include-book "tools/trivial-ancestors-check" :dir :system))
-  (local (acl2::use-trivial-ancestors-check))
-
-  ;; (defthm rational-exponent-when-expt*2-less
-  ;;   (implies (and (rationalp x)
-  ;;                 (<= (* 2 (expt 2 i)) x)
-  ;;                 (integerp i))
-  ;;            (<= (+ 1 i) (acl2::rational-exponent x)))
-  ;;   :hints (("goal" :use ((:instance rational-exponent-when-expt-less
-  ;;                          (i (+ 1 i)) (x x)))
-  ;;            :expand ((expt 2 (+ 1 i)))
-  ;;            :in-theory (disable rational-exponent-when-expt-less)
-  ;;            :do-not-induct t))
-  ;;   :rule-classes :linear)
-
-  (defthm rational-exponent-when-expt-strictly-less
-    (implies (and (rationalp x)
-                  (< (expt 2 i) x)
-                  (integerp i))
-             (<= i (acl2::rational-exponent x)))
-    :hints (("goal" :use ((:instance rational-exponent-when-expt-less
-                           (i i) (x x)))
-             :in-theory (disable rational-exponent-when-expt-less)
-             :do-not-induct t))
-    :rule-classes :linear)
-  
-  (defthm log2-loop-correct
-    (b* ((storage (local-env->storage
-                   (env->local env)))
-         (a-look (assoc-equal "__stdlib_local_a" storage))
-         (a (cdr a-look))
-         ((v_int a))
-         (current-look (assoc-equal "__stdlib_local_current" storage))
-         (current (cdr current-look))
-         ((v_int current))
-         (result-look (assoc-equal "__stdlib_local_result" storage))
-         (result (cdr result-look))
-         ((v_int result)))
-      (implies (and a-look
-                    (val-case a :v_int)
-                    current-look
-                    (val-case current :v_int)
-                    result-look
-                    (val-case result :v_int)
-                    (<= 0 result.val)
-                    (equal current.val (expt 2 result.val))
-                    (< current.val (* 2 a.val))
-                    (natp clk)
-                    (< (- (+ 1 (acl2::rational-exponent a.val)) result.val) clk)
-                    (integerp limit)
-                    (< (- (+ 1 (acl2::rational-exponent a.val)) result.val) limit)
-                    (no-duplicatesp-equal (acl2::alist-keys storage)))
-               (b* (((mv (ev_normal res) &) (eval_loop env t limit *log2-loop-test* *log2-loop-body*))
-                    ((continuing res.res))
-                    (result-spec (let ((exp (acl2::rational-exponent a.val)))
-                                   (if (equal a.val (expt 2 exp))
-                                       exp
-                                     (+ 1 exp))))
-                    (current-spec (expt 2 result-spec))
-                    ((env env))
-                    ((local-env env.local)))
-                 (and (equal (eval_result-kind res) :ev_normal)
-                      (equal (control_flow_state-kind res.res) :continuing)
-                      (equal res.res.env
-                             (change-env env
-                                         :local (change-local-env
-                                                 env.local
-                                                 :storage (put-assoc-equal "__stdlib_local_current"
-                                                                           (v_int current-spec)
-                                                                           (put-assoc-equal "__stdlib_local_result"
-                                                                                            (v_int result-spec)
-                                                                                            env.local.storage)))))))))
-    :hints (("goal" :induct (loop-induct env clk *log2-loop-test* *log2-loop-body* t limit orac)
-             :in-theory (enable check_recurse_limit
-                                declare_local_identifiers
-                                declare_local_identifier
-                                env-find
-                                env-assign
-                                env-assign-local
-                                env-assign-global
-                                env-push-stack
-                                env-pop-stack
-                                pop_scope
-                                tick_loop_limit
-                                v_to_bool)
-             :do-not-induct t)
-            (and stable-under-simplificationp
-                 '(:expand ((eval_loop env t limit *log2-loop-test* *log2-loop-body*))))
-            (and stable-under-simplificationp
-                 '(:use ((:instance rational-exponent-hack
-                          (a (V_INT->VAL
-                              (CDR (HONS-ASSOC-EQUAL "__stdlib_local_a"
-                                                     (LOCAL-ENV->STORAGE (ENV->LOCAL ENV))))))
-                          (r (V_INT->VAL
-                              (CDR (HONS-ASSOC-EQUAL "__stdlib_local_result"
-                                                     (LOCAL-ENV->STORAGE (ENV->LOCAL ENV))))))))
-                   :in-theory (e/d (equal-when-v_int)
-                                   (equal-of-v_int)
-                                   ))))))
 
 
 (defsection log2-correct
