asllib/acl2/proofs/stdlib/uint.lisp
@@ -36,113 +36,38 @@
                            bitops::part-select)))
 
 
-
-
-
-(defsection uint-loop
-
-  (local (defthm ash-of-partselect-plus-one
-           (implies (natp start)
-                    (equal (ash (bitops::part-select-width-low val width (+ 1 start)) (+ 1 start))
-                           (- (ash (bitops::part-select-width-low val (+ 1 (nfix width)) start) start)
-                              (* (logbit start val) (expt 2 start)))))
-           :hints(("Goal" :in-theory (enable bitops::ash-is-expt-*-x
-                                             bitops::part-select-width-low
-                                             logcons)
-                   :expand ((logtail (+ 1 start) val)
-                            (:free (x) (loghead (+ 1 (nfix width)) x)))))))
+(defloop uint-loop
+  :function "UInt"
+  :looptype :s_for
+  :local-vars (((v_bitvector x) "__stdlib_local_x")
+               ((v_int n) "__stdlib_local_N")
+               ((v_int result) "__stdlib_local_result"
+                (v_int (+ result.val (ash (bitops::part-select x.val :low start :high end) start)))))
+  :index-var i
+  :invariants (and (<= 0 start)
+                   (<= (+ 1 end) x.len))
+  :prepwork
+  ((local (defthm ash-of-partselect-plus-one
+            (implies (natp start)
+                     (equal (ash (bitops::part-select-width-low val width (+ 1 start)) (+ 1 start))
+                            (- (ash (bitops::part-select-width-low val (+ 1 (nfix width)) start) start)
+                               (* (logbit start val) (expt 2 start)))))
+            :hints(("Goal" :in-theory (enable bitops::ash-is-expt-*-x
+                                              bitops::part-select-width-low
+                                              logcons)
+                    :expand ((logtail (+ 1 start) val)
+                             (:free (x) (loghead (+ 1 (nfix width)) x)))))))
   
-  (local (defthm loghead-of-part-select
-           (implies (<= (nfix n) (nfix width))
-                    (equal (loghead n (bitops::part-select-width-low val width low))
-                           (loghead n (logtail low val))))
-           :hints(("Goal" :in-theory (enable bitops::part-select-width-low)))))
+   (local (defthm loghead-of-part-select
+            (implies (<= (nfix n) (nfix width))
+                     (equal (loghead n (bitops::part-select-width-low val width low))
+                            (loghead n (logtail low val))))
+            :hints(("Goal" :in-theory (enable bitops::part-select-width-low)))))
 
 
-  (local (defthm part-select-0-width
-           (equal (bitops::part-select-width-low val 0 low) 0)
-           :hints(("Goal" :in-theory (enable bitops::part-select-width-low)))))
-  
-  (defconst *uint-loop*
-    (find-nth-form 0 :s_for (assoc-equal "UInt" (static_env_global->subprograms
-                                                 (stdlib-static-env)))))
-
-  (defconst *uint-loop-body*
-    (s_for->body *uint-loop*))
-
-  (defthm uint-loop-correct
-    (b* ((storage (local-env->storage
-                   (env->local env)))
-         (i-look (assoc-equal "__stdlib_local_i" storage))
-         (i (cdr i-look))
-         ((v_int i))
-         (x-look (assoc-equal "__stdlib_local_x" storage))
-         (x (cdr x-look))
-         ((v_bitvector x))
-         (N-look (assoc-equal "__stdlib_local_N" storage))
-         (N (cdr N-look))
-         ((v_int N))
-         (result-look (assoc-equal "__stdlib_local_result" storage))
-         (result (cdr result-look))
-         ((v_int result)))
-      (implies (and i-look
-                    (val-case i :v_int)
-                    (equal i.val start)
-                    x-look
-                    (val-case x :v_bitvector)
-                    N-look
-                    (val-case N :v_int)
-                    result-look
-                    (val-case result :v_int)
-
-                    (natp clk)
-                    (natp start)
-                    (integerp end)
-                    (<= start (+ 1 end))
-                    (<= (+ 1 end) x.len)
-                    (no-duplicatesp-equal (acl2::alist-keys storage)))
-               (b* (((mv (ev_normal res) &) (eval_for env "__stdlib_local_i" nil start :up end *uint-loop-body*))
-                    ((continuing res.res))
-                    (result-spec (+ result.val (ash (bitops::part-select x.val :low start :high end) start)))
-                    ((env env))
-                    ((local-env env.local)))
-                 (and (equal res.res.env
-                             (change-env env
-                                         :local (change-local-env
-                                                 env.local
-                                                 :storage (put-assoc-equal "__stdlib_local_i"
-                                                                           (v_int (+ 1 end))
-                                                                           (put-assoc-equal "__stdlib_local_result"
-                                                                                            (v_int result-spec)
-                                                                                            env.local.storage)))))
-                      (equal (eval_result-kind res) :ev_normal)
-                      (equal (control_flow_state-kind res.res) :continuing)))))
-    :hints (("goal" :induct (for-induct env "__stdlib_local_i" start :up end *uint-loop-body* clk nil orac)
-             :in-theory (enable check_recurse_limit
-                                declare_local_identifiers
-                                declare_local_identifier
-                                env-find
-                                env-assign
-                                env-assign-local
-                                env-assign-global
-                                env-push-stack
-                                env-pop-stack
-                                eval_for_step
-                                for_loop-step
-                                FOR_LOOP-TEST
-                                pop_scope
-                                check-bad-slices
-                                slices_sub)
-             :do-not-induct t)
-            (and stable-under-simplificationp
-                 '(:expand ((eval_for env "__stdlib_local_i"
-                                      nil
-                                      (V_INT->VAL
-                                       (CDR (HONS-ASSOC-EQUAL "__stdlib_local_i"
-                                                              (LOCAL-ENV->STORAGE (ENV->LOCAL ENV)))))
-                                      :up end *uint-loop-body*)
-                            (eval_for env "__stdlib_local_i" nil end :up end *uint-loop-body*)
-                            (eval_for env "__stdlib_local_i" nil (+ 1 end) :up end *uint-loop-body*)))))))
+   (local (defthm part-select-0-width
+            (equal (bitops::part-select-width-low val 0 low) 0)
+            :hints(("Goal" :in-theory (enable bitops::part-select-width-low)))))))
 
 
 
